src/program_proof/tulip/program/backup/backup.v
@@ -1,0 +1,180 @@
+From Perennial.program_proof.tulip.program Require Import prelude.
+
+Section repr.
+  Context `{!heapGS Σ, !tulip_ghostG Σ}.
+
+  Definition own_tcoord (tcoord : loc) (ts : nat) (γ : tulip_names) : iProp Σ.
+  Admitted.
+
+End repr.
+
+Section repr.
+  Context `{!heapGS Σ, !tulip_ghostG Σ}.
+
+  Theorem wp_BackupTxnCoordinator__stabilize tcoord ts γ :
+    {{{ own_tcoord tcoord ts γ }}}
+      BackupTxnCoordinator__stabilize #tcoord
+    {{{ (status : txnphase) (valid : bool), RET (#(txnphase_to_u64 status), #valid); 
+        own_tcoord tcoord ts γ ∗
+        if valid then safe_txnphase γ ts status else True
+    }}}.
+  Proof.
+    (*@ func (tcoord *BackupTxnCoordinator) stabilize() (uint64, bool) {        @*)
+    (*@     ts := tcoord.ts                                                     @*)
+    (*@     rank := tcoord.rank                                                 @*)
+    (*@     ptgs := tcoord.ptgs                                                 @*)
+    (*@                                                                         @*)
+    (*@     mu := new(sync.Mutex)                                               @*)
+    (*@     cv := sync.NewCond(mu)                                              @*)
+    (*@     // Number of groups that have responded (i.e., groups whose prepare status @*)
+    (*@     // is determined).                                                  @*)
+    (*@     var nr uint64 = 0                                                   @*)
+    (*@     // Number of groups that have prepared.                             @*)
+    (*@     var np uint64 = 0                                                   @*)
+    (*@     var st uint64 = tulip.TXN_PREPARED                                  @*)
+    (*@     var vd bool = true                                                  @*)
+    (*@                                                                         @*)
+    (*@     for _, gcoordloop := range(tcoord.gcoords) {                        @*)
+    (*@         gcoord := gcoordloop                                            @*)
+    (*@                                                                         @*)
+    (*@         go func() {                                                     @*)
+    (*@             stg, vdg := gcoord.Prepare(ts, rank, ptgs)                  @*)
+    (*@                                                                         @*)
+    (*@             mu.Lock()                                                   @*)
+    (*@             nr += 1                                                     @*)
+    (*@             if !vdg {                                                   @*)
+    (*@                 vd = false                                              @*)
+    (*@             } else if stg == tulip.TXN_PREPARED {                       @*)
+    (*@                 np += 1                                                 @*)
+    (*@             } else {                                                    @*)
+    (*@                 st = stg                                                @*)
+    (*@             }                                                           @*)
+    (*@             mu.Unlock()                                                 @*)
+    (*@             cv.Signal()                                                 @*)
+    (*@         }()                                                             @*)
+    (*@     }                                                                   @*)
+    (*@                                                                         @*)
+    (*@     // Wait until either a higher-ranked coordinator is found (i.e., as @*)
+    (*@     // indicated by @valid = false), or all participant groups have responded. @*)
+    (*@     //                                                                  @*)
+    (*@     // A note on the difference between this method and @txn.preapre. Unlike @*)
+    (*@     // @txn.prepare() where it's OK (and good for performance) to terminate this @*)
+    (*@     // phase once the transaction status is determined, the backup txn  @*)
+    (*@     // coordinator should wait until it finds out the status of all participant @*)
+    (*@     // groups to finalize the transaction outcome for every group.      @*)
+    (*@     mu.Lock()                                                           @*)
+    (*@     for vd && nr != uint64(len(tcoord.gcoords)) {                       @*)
+    (*@         cv.Wait()                                                       @*)
+    (*@     }                                                                   @*)
+    (*@                                                                         @*)
+    (*@     // Use the invariant saying that "if @st = TXN_PREPARED, then @np = @nr" to @*)
+    (*@     // establish the postcondition.                                     @*)
+    (*@                                                                         @*)
+    (*@     status := st                                                        @*)
+    (*@     valid := vd                                                         @*)
+    (*@     mu.Unlock()                                                         @*)
+    (*@                                                                         @*)
+    (*@     return status, valid                                                @*)
+    (*@ }                                                                       @*)
+  Admitted.
+
+  Theorem wp_BackupTxnCoordinator__abort tcoord ts γ :
+    is_txn_aborted γ ts -∗
+    {{{ own_tcoord tcoord ts γ }}}
+      BackupTxnCoordinator__abort #tcoord
+    {{{ RET #(); own_tcoord tcoord ts γ }}}.
+  Proof.
+    (*@ func (tcoord *BackupTxnCoordinator) abort() {                           @*)
+    (*@     for _, gcoordloop := range(tcoord.gcoords) {                        @*)
+    (*@         gcoord := gcoordloop                                            @*)
+    (*@         go func() {                                                     @*)
+    (*@             gcoord.Abort(tcoord.ts)                                     @*)
+    (*@         }()                                                             @*)
+    (*@     }                                                                   @*)
+    (*@ }                                                                       @*)
+  Admitted.
+
+  Theorem wp_BackupTxnCoordinator__resolve tcoord status ts γ :
+    status ≠ TxnAborted ->
+    {{{ own_tcoord tcoord ts γ }}}
+      BackupTxnCoordinator__resolve #tcoord #(txnphase_to_u64 status)
+    {{{ RET #(); own_tcoord tcoord ts γ ∗ is_txn_committed_ex γ ts }}}.
+  Proof.
+    (*@ func (tcoord *BackupTxnCoordinator) resolve(status uint64) {            @*)
+    (*@     if status == tulip.TXN_PREPARED {                                   @*)
+    (*@         // Logical action: Commit.                                      @*)
+    (*@         trusted_proph.ResolveCommit(tcoord.proph, tcoord.ts, tcoord.mergeWrites()) @*)
+    (*@     }                                                                   @*)
+    (*@ }                                                                       @*)
+  Admitted.
+
+  Theorem wp_BackupTxnCoordinator__commit tcoord ts γ :
+    is_txn_committed_ex γ ts -∗
+    {{{ own_tcoord tcoord ts γ }}}
+      BackupTxnCoordinator__commit #tcoord
+    {{{ RET #(); own_tcoord tcoord ts γ }}}.
+  Proof.
+    (*@ func (tcoord *BackupTxnCoordinator) commit() {                          @*)
+    (*@     for _, gcoordloop := range(tcoord.gcoords) {                        @*)
+    (*@         gcoord := gcoordloop                                            @*)
+    (*@         go func() {                                                     @*)
+    (*@             gcoord.Commit(tcoord.ts)                                    @*)
+    (*@         }()                                                             @*)
+    (*@     }                                                                   @*)
+    (*@ }                                                                       @*)
+  Admitted.
+
+  Theorem wp_BackupTxnCoordinator__Finalize tcoord ts γ :
+    {{{ own_tcoord tcoord ts γ }}}
+      BackupTxnCoordinator__Finalize #tcoord
+    {{{ RET #(); own_tcoord tcoord ts γ }}}.
+  Proof.
+    iIntros (Φ) "Htcoord HΦ".
+    wp_rec.
+
+    (*@ func (tcoord *BackupTxnCoordinator) Finalize() {                        @*)
+    (*@     status, valid := tcoord.stabilize()                                 @*)
+    (*@                                                                         @*)
+    wp_apply (wp_BackupTxnCoordinator__stabilize with "Htcoord").
+    iIntros (status valid) "[Htcoord Hphase]".
+    wp_pures.
+    
+    (*@     if !valid {                                                         @*)
+    (*@         // Skip since a more recent backup txn coordinator is found.    @*)
+    (*@         return                                                          @*)
+    (*@     }                                                                   @*)
+    (*@                                                                         @*)
+    destruct valid eqn:Hvalid; wp_pures; last first.
+    { by iApply "HΦ". }
+
+    (*@     if status == tulip.TXN_ABORTED {                                    @*)
+    (*@         tcoord.abort()                                                  @*)
+    (*@         return                                                          @*)
+    (*@     }                                                                   @*)
+    (*@                                                                         @*)
+    case_bool_decide as Hcond; wp_pures.
+    { destruct status eqn:Hstatus; [done | done | ].
+      simpl.
+      wp_apply (wp_BackupTxnCoordinator__abort with "Hphase Htcoord").
+      iIntros "Htcoord".
+      wp_pures.
+      by iApply "HΦ".
+    }
+
+    (*@     // Possible @status: TXN_PREPARED and TXN_COMMITTED. Resolve the prophecy @*)
+    (*@     // variable if @status == TXN_PREPARED.                             @*)
+    (*@     tcoord.resolve(status)                                              @*)
+    (*@                                                                         @*)
+    wp_apply (wp_BackupTxnCoordinator__resolve with "Htcoord").
+    { by destruct status. }
+    iIntros "[Htcoord #Hcmted]".
+
+    (*@     tcoord.commit()                                                     @*)
+    (*@ }                                                                       @*)
+    wp_apply (wp_BackupTxnCoordinator__commit with "Hcmted Htcoord").
+    iIntros "Htcoord".
+    wp_pures.
+    by iApply "HΦ".
+  Qed.
+
+End repr.
